examples/algorithms/IntSort.fst
@@ -1,5 +1,5 @@
 module IntSort
-open FStar.List
+open FStar.List.Tot
 
 (* Check that a list is sorted *)
 val sorted: list int -> Tot bool
@@ -27,9 +27,9 @@ let rec sorted_smaller x y l = match l with
     | z::zs -> if z=y then () else sorted_smaller x y zs
 
 
-opaque type permutation (l1:list int) (l2:list int) =
+type permutation (l1:list int) (l2:list int) =
     length l1 = length l2 /\ (forall n. mem n l1 = mem n l2)
 
-opaque type permutation_2 (l:list int) (l1:list int) (l2:list int) =
+type permutation_2 (l:list int) (l1:list int) (l2:list int) =
     (forall n. mem n l = (mem n l1 || mem n l2)) /\
     length l = length l1 + length l2
