examples/algorithms/MergeSort.fst
@@ -1,8 +1,8 @@
 module MergeSort
-open FStar.List
+open FStar.List.Tot
 open IntSort
 
-opaque type split_inv (l:list int) (l1:list int) (l2:list int) =
+type split_inv (l:list int) (l1:list int) (l2:list int) =
     permutation_2 l l1 l2 /\
     (* needed for decreases clause in mergesort function *)
     length l > length l1 /\ length l > length l2
@@ -19,7 +19,7 @@ let rec split (x::y::l) =
 
 (* Verification succeeds even without this invariant;
    it just takes a lot longer (22s vs 7s) *)
-opaque type merge_inv (l1:list int) (l2:list int) (l:list int) =
+type merge_inv (l1:list int) (l2:list int) (l:list int) =
     (is_Cons l1 /\ is_Cons l /\ Cons.hd l1 = Cons.hd l) \/
     (is_Cons l2 /\ is_Cons l /\ Cons.hd l2 = Cons.hd l) \/
     (is_Nil l1 /\ is_Nil l2 /\ is_Nil l)
