ulib/FStar.Array.fst
@@ -90,9 +90,9 @@ val copy_aux:
 			      /\ (modifies !{cpy} h0 h1)
 			      /\ (Seq.equal (sel h1 cpy) (sel h1 s))))
 let rec copy_aux #a s cpy ctr =
-  match Array.length cpy - ctr with
+  match length cpy - ctr with
   | 0 -> ()
-  | _ -> Array.upd cpy ctr (Array.index s ctr);
+  | _ -> upd cpy ctr (index s ctr);
 	 copy_aux s cpy (ctr+1)
 
 val copy:
@@ -105,7 +105,7 @@ val copy:
 				     /\ (contains h1 r)
 				     /\ (Seq.equal (sel h1 r) (sel h0 s))))
 let copy #a s =
-  let cpy = Array.create (Array.length s) (Array.index s 0) in
+  let cpy = create (length s) (index s 0) in
   copy_aux s cpy 0;
   cpy
 
@@ -134,7 +134,7 @@ val blit_aux:
 let rec blit_aux #a s s_idx t t_idx len ctr =
   match len - ctr with
   | 0 -> ()
-  | _ -> Array.upd t (t_idx + ctr) (Array.index s (s_idx + ctr));
+  | _ -> upd t (t_idx + ctr) (index s (s_idx + ctr));
 	 blit_aux s s_idx t t_idx len (ctr+1)
 
 val blit:
@@ -177,6 +177,6 @@ val sub :
       /\ (idx + len <= Seq.length (sel h0 s))
       /\ (Seq.equal (Seq.slice (sel h0 s) idx (idx+len)) (sel h1 t))))
 let sub #a s idx len =
-  let t = Array.create len (index s 0) in
-  Array.blit s idx t 0 len;
+  let t = create len (index s 0) in
+  blit s idx t 0 len;
   t
